refactored

red-black-tree.dfy
@@ -1,16 +1,6 @@
 // https://dafny-lang.github.io/dafny/DafnyRef/DafnyRef#1910-binding-guards
 
-// do imperative BST instead of full-fledged RBTree
-
 datatype Color = Red | Black
-
-// datatype RBTree = Empty  | Node (color : Color, value : int, left : RBTree, right : RBTree)
-
-// function method elems(t : RBTree) : set<int> {
-// 	if t == Empty then {} else {t.value} + elems(t.left) + elems(t.right)
-// }
-
-
 // twostate lemma ValidFix(x : RBTreeRef, y : RBTreeRef)
 // 	requires y.parent == old(y.parent)
 // 	requires y.Repr == old(y.Repr)
@@ -58,43 +48,96 @@ class RBTreeRef {
 		}
 
 
-		predicate Valid()
+		function method elems() : set<int>
+			reads this, Repr
+			requires ValidWeak()
 			decreases Repr
-			ensures Valid() ==>  ValidWeak() && isOrdered(Tree) && isBalanced(Tree)
-  		reads this, Repr {
-				this in Repr &&
-					Tree.Node? &&
-					Tree.value == value &&
-					Tree.color == color &&
-					(left == null ==> Tree.left.Empty?) &&
-					(right == null ==> Tree.right.Empty?) &&
-					(left != null ==> left in Repr && left.Repr <= Repr && this !in left.Repr &&
-					left.Valid() && left.Tree == Tree.left && left.parent == this) &&
-					(right != null ==> right in Repr && right.Repr <= Repr && this !in right.Repr &&
-					right.Valid() && right.Tree == Tree.right && right.parent == this) &&
-					(left != null && right != null ==> left.Repr * right.Repr == {}) &&
-					// isWellFormed(Tree)
-					isBalanced(Tree) &&
-					isOrdered(Tree)
+		{
+			{value} + (if left != null then left.elems() else {}) + (if right != null then right.elems() else {})
 		}
 
+		predicate isOrdered()
+			reads this, Repr
+			requires ValidWeak()
+			decreases Repr
+		{
+			(left != null ==> left.isOrdered() && forall i :: i  in left.elems() ==> i < value) &&
+				(right != null ==> right.isOrdered() && forall i :: i  in right.elems() ==> i > value)
+		}
+
+		function countBlack() : int
+			reads this, Repr
+			requires ValidWeak()
+			decreases Repr
+		{
+			(if color == Black then 1 else 0) + (if left == null then 1 else left.countBlack())
+				// no right. this is NOT a typo
+		}
+
+
+    predicate isBalanced()
+			reads this, Repr
+			requires ValidWeak()
+		{
+			countBlackN(left) == countBlackN(right) &&
+				(left != null ==> left.isBalanced()) &&
+				(right != null ==> right.isBalanced())
+		}
+
+		predicate isNoRedRed()
+			reads this, Repr
+			requires ValidWeak()
+		{
+			(left != null ==> left.isNoRedRed() && (color == Red ==> left.color == Red)) &&
+				(right != null ==> right.isNoRedRed() && (color == Red ==> right.color == Red))
+		}
+
+		predicate isNoRedRedL()
+			reads this, Repr
+			requires ValidWeak()
+		{
+			(left != null ==> left.isNoRedRed() && (color == Red ==> left.color == Red)) &&
+				(right != null ==> (color == Red ==> right.color == Red))
+		}
+
+
+		predicate isNoRedRedR()
+			reads this, Repr
+			requires ValidWeak()
+		{
+			(left != null ==> (color == Red ==> left.color == Red)) &&
+				(right != null ==> right.isNoRedRed() && (color == Red ==> right.color == Red))
+		}
+
+		predicate isNoRedRedRP()
+			reads this, Repr
+			requires ValidWeak()
+		{
+				(right != null ==> right.isNoRedRed() && (color == Red ==> right.color == Red))
+		}
+
+		predicate isNoRedRedLP()
+			reads this, Repr
+			requires ValidWeak()
+		{
+			(left != null ==> left.isNoRedRed() && (color == Red ==> left.color == Red))
+		}
+		
 
 		predicate ValidRB()
-			decreases Repr
-			ensures Valid() && noRedRed(Tree) <==> ValidRB()
-			// ensures ValidRB() ==> Valid()
-  		reads this, Repr {
-				this in Repr &&
-					(left != null ==> left in Repr && left.Repr <= Repr && this !in left.Repr &&
-					left.ValidRB() && left.Tree == Tree.left && left.parent == this) &&
-					(right != null ==> right in Repr && right.Repr <= Repr && this !in right.Repr &&
-					right.ValidRB() && right.Tree == Tree.right && right.parent == this) &&
-					(left != null && right != null ==> left.Repr * right.Repr == {}) &&
-					// isWellFormed(Tree)
-					isBalanced(Tree) &&
-					isOrdered(Tree) &&
-					noRedRed(Tree)
+			reads this, Repr
+			requires ValidWeak()
+	  {
+			ValidWeak() && isNoRedRed() && isBalanced() && isOrdered()
 		}
+
+		predicate Valid()
+			reads this, Repr
+			requires ValidWeak()
+	  {
+			ValidWeak() && isBalanced() && isOrdered()
+		}
+
 
 		// termination metric
 		static function ReprN (t : RBTreeRef?) : set<RBTreeRef>
@@ -104,8 +147,8 @@ class RBTreeRef {
 
 
 		static method Member(t : RBTreeRef?, v : int) returns (r : bool)
-			requires t != null ==> t.Valid()
-			ensures (t == null ==> !r) && (t != null ==> (r <==> v in elems(t.Tree)))
+			requires t != null ==> t.ValidWeak() && t.Valid()
+			ensures (t == null ==> !r) && (t != null ==> (r <==> v in t.elems()))
 			decreases ReprN(t)
 		{
 			if (t == null) {
@@ -125,13 +168,13 @@ class RBTreeRef {
 			}
 		}
 
-		static method getParent(t : RBTreeRef?) returns (p : RBTreeRef?) {
-			if (t == null) {
-				return null;
-			}
+		// static method getParent(t : RBTreeRef?) returns (p : RBTreeRef?) {
+		// 	if (t == null) {
+		// 		return null;
+		// 	}
 
-			return t.parent;
-		}
+		// 	return t.parent;
+		// }
 
 		// static method getRoot(t :RBTreeRef) returns (p : RBTreeRef?) {
 		// 	if (t.parent == null) {
@@ -142,14 +185,10 @@ class RBTreeRef {
 		// }
 
 		static function ElemsN (t : RBTreeRef?) : set<int>
-		reads t {
-			if (t == null) then {} else elems(t.Tree)
-		}
-
-
-		static function countBlackN (t : RBTreeRef?) : int
-			reads t {
-				if (t == null) then 1 else countBlack(t.Tree)
+			reads t, ReprN(t)
+			requires t != null ==> t.ValidWeak()
+    {
+			if (t == null) then {} else t.elems()
 		}
 
 
@@ -163,21 +202,6 @@ class RBTreeRef {
 				{this} + (if left == null then {} else left.ElemsRef()) + (if right == null then {} else right.ElemsRef())
 		}
 
-		// function AncestorsRef () : set<RBTreeRef>
-		// 	decreases this.ReprP
-		// 	reads this, this.ReprP
-		// 	requires this.ValidWeakP()
-		// 	ensures this.AncestorsRef() <= this.ReprP
-			
-		// 	// ensures this.ElemsRef() <= this.Repr
-		// 	ensures forall i :: i in AncestorsRef() ==> i.ValidWeakP() && i in this.ReprP
-		// 	// ensures forall i :: i in AncestorsRef() && i != this ==> i.ReprP < ReprP &&  i.parent != null && i.parent in AncestorsRef() && i.ReprP < i.parent.ReprP
-		// {
-		// 	{this} + (if parent == null then {} else parent.AncestorsRef())
-		// }
-
-
-		
 
 		predicate PartialNoRR (root : RBTreeRef)
 			reads root, root.Repr
@@ -188,23 +212,26 @@ class RBTreeRef {
 			this != root ==>
 				this.parent.PartialNoRR(root) &&
 				(this.parent.left == this || this.parent.right == this) &&
-				(this.parent.left == this ==> noRedRedR(this.parent.Tree)) &&
-				(this.parent.right == this ==> noRedRedL(this.parent.Tree))
+				(this.parent.left == this ==> this.parent.isNoRedRedR()) &&
+				(this.parent.right == this ==> this.parent.isNoRedRedL())
 		}
 
-
 		predicate PartialNoRRP ()
-			reads this.parent
-			reads this
-			requires this.parent != null
+			requires parent != null ==> parent.ValidWeak()
+			reads this, this.parent, ReprN(this.parent)
+			// requires this in root.ElemsRef()
+			// decreases root.Repr - this.Repr
 		{
-			  (this.parent.left == this || this.parent.right == this) &&
-				(this.parent.left == this ==> noRedRedRP(this.parent.Tree)) &&
-				(this.parent.right == this ==> noRedRedLP(this.parent.Tree))
+			this.parent != null ==>
+				(this.parent.left == this || this.parent.right == this) &&
+				(this.parent.left == this ==> this.parent.isNoRedRedRP()) &&
+				(this.parent.right == this ==> this.parent.isNoRedRedLP())
 		}
 
 
 		static lemma CombineNoRR(r0 : RBTreeRef, r1 : RBTreeRef)
+			requires r0.ValidWeak()
+			requires r1.ValidWeak()
 			requires r0.ValidRB()
 			requires r1.Valid()
 			requires r0 in r1.ElemsRef()
@@ -224,8 +251,10 @@ class RBTreeRef {
 
 
 		static lemma ElemsRefTrans(r0 : RBTreeRef, r1 : RBTreeRef, r2 : RBTreeRef)
-			requires r1.Valid()
-			requires r2.Valid()
+			requires r1.ValidWeak()
+			requires r2.ValidWeak()
+			// requires r1.Valid()
+			// requires r2.Valid()
 			requires r0 in r1.ElemsRef()
 			requires r1 in r2.ElemsRef()
 			decreases r2.Repr
@@ -245,10 +274,19 @@ class RBTreeRef {
 			ElemsRefTrans(r0,r1,r2.left);
 		}
 
-		// // use convert?
-		static ghost method partialNoRRTrans(r0 : RBTreeRef, r1 : RBTreeRef, r2 : RBTreeRef)
-			requires r1.Valid()
-			requires r2.Valid()
+		static function countBlackN(r0:RBTreeRef?) : int
+			reads r0, ReprN(r0)
+			requires r0 != null ==> r0.ValidWeak()
+		{
+			if r0 == null then 1 else r0.countBlack()
+		}
+
+  		// // // use convert?
+ 		static ghost method partialNoRRTrans(r0 : RBTreeRef, r1 : RBTreeRef, r2 : RBTreeRef)
+  		requires r1.ValidWeak()
+  		requires r2.ValidWeak()
+			// requires r1.Valid()
+			// requires r2.Valid()
 			decreases r1.Repr - r0.Repr
 			requires r0 in r1.ElemsRef()
 			requires r1 in r2.ElemsRef()
@@ -257,16 +295,12 @@ class RBTreeRef {
 			requires r1.PartialNoRR(r2)
 			ensures r0.PartialNoRR(r2)
 			{
-				if(r0==r1) {
-					assert(r0.PartialNoRR(r2));
-					return;
+				if(r0!=r1) {
+					partialNoRRTrans(r0.parent, r1, r2);
 				}
+			}
 
-				assert(r0.parent in r1.ElemsRef());
-				assert(r0.parent.PartialNoRR(r1));
-				partialNoRRTrans(r0.parent, r1, r2);
-			// assert(r1 != r2);
-		}
+
 
     // http://leino.science/papers/krml273.html
 		// static method insert(t : RBTreeRef?, v : int) returns (r : RBTreeRef)
@@ -423,300 +457,113 @@ class RBTreeRef {
 		// 	}
 		// }
 
-		// static method insertBST(t : RBTreeRef?, n : RBTreeRef) returns (r : RBTreeRef)
-		// 	requires n.parent == null
-		// 	requires n.Repr == {n}
-		// 	requires n !in ReprN(t)
-		// 	requires t != null ==> t.ValidRB()
-		// 	requires n.Valid()
-		// 	requires elems(n.Tree)=={n.value}
-		// 	requires n.color == Red
+		static method insertBST(t : RBTreeRef?, n : RBTreeRef) returns (r : RBTreeRef)
+			requires n.parent == null
+			requires n.Repr == {n}
+			requires n !in ReprN(t)
+			requires t != null ==> t.ValidWeak() && t.ValidRB()
+			requires n.ValidWeak()
+			requires n.Valid()
+			requires n.left == null && n.right == null && n.color == Red
+			requires n.color == Red
 
- 		// 	modifies if t != null then t.Repr else {}
-		// 	modifies n`parent
+ 			modifies if t != null then t.Repr else {}
+			modifies n`parent
 				
-  	// 	ensures if t == null then r == n else r == t
-		// 	ensures t != null ==> t.parent == old(t.parent)
-		// 	ensures n.ValidRB()
-		// 	ensures t != null ==> old(ElemsN(t)) + {n.value} == ElemsN(t)
-		// 	ensures ElemsN(r) == ElemsN(t) + {n.value}
-		// 	ensures old(countBlackN(t)) == countBlackN(r)
-		// 	ensures t != null ==> old(t.Repr) + {n} == r.Repr
-		// 	ensures r.Valid()
-		// 	ensures n.parent != null ==> n in r.ElemsRef() && (n != r ==> n.parent.PartialNoRR(r)) && n.PartialNoRRP()
-		// 	ensures t == r ==> t.color == old(t.color)
-		// 	ensures (n.parent == null && n != r) ==> r == t && t.color == old(t.color) &&
-		// 	          t.value == old(t.value) && t.left == old(t.left) && t.right == old(t.right) && t.Tree == old(t.Tree)
-    //   decreases ReprN(t)
-		// {
+			ensures n.Repr == old(n.Repr) && n.value == old(n.value) && n.left == null && n.right == null && n.color == Red
+			ensures t != null ==> t.ValidWeak() && old(t.Repr) + {n} == r.Repr && t == r && t.color == old(t.color) && old(t.elems()) + {n.value} == t.elems()
+  		ensures if t == null then r == n else r == t
+			ensures t != null ==> t.parent == old(t.parent)
+			ensures r.ValidWeak()
+			ensures n.ValidWeak()
+			ensures n.ValidRB()
+			ensures (n.parent == null && n != r) ==> r == t && t.color == old(t.color) &&
+			          t.value == old(t.value) && t.left == old(t.left) && t.right == old(t.right)
+			ensures t != null ==> old(ElemsN(t)) + {n.value} == ElemsN(t)
+			ensures ElemsN(r) == ElemsN(t) + {n.value}
+			ensures old(countBlackN(t)) == countBlackN(r)
+			ensures r.Valid()
+			ensures n.parent != null ==> n.parent.ValidWeak()
+			ensures n.parent != null ==> n in r.ElemsRef() && (n != r ==> n.parent.PartialNoRR(r)) && n.PartialNoRRP()
+      decreases ReprN(t)
+		{
 
-		// 	if (t == null) {
-		// 		r := n;
-		// 		return;
-		// 	}
+			if (t == null) {
+				r := n;
+				return;
+			}
 
-		// 	r := t;
+			r := t;
 
-		// 	if (t.value == n.value) {
-		// 		t.Repr := t.Repr + {n};
-		// 		return;
-		// 	}
-
-
-		// 	// n.parent doesn't work because dafny doesn't know n remains the same
-
-		// 	if (n.value < t.value) {
-
-		// 		var newLeft := insertBST(t.left, n);
-
-		// 		r.Repr := r.Repr + {n};
-		// 		r.Tree := Node(t.color,t.value,newLeft.Tree,t.Tree.right);
-		// 		r.left := newLeft;
-		// 		if(newLeft == n){
-		// 			n.parent := t;
-		// 		}
-
-		// 		if(n.parent != null){
-		// 			ElemsRefTrans(n,newLeft,r);
-		// 			if(n != newLeft) {
-		// 				partialNoRRTrans(n.parent,newLeft,r);
-		// 			}
-
-		// 		assert(n.parent in r.ElemsRef());
-		// 		}
-		// 		return;
-		// 	}
-
-		// 	if (n.value > t.value) {
-		// 		var newRight := insertBST(t.right, n);
-		// 		r.Repr := r.Repr + {n};
-		// 		r.Tree := Node(t.color,t.value,t.Tree.left,newRight.Tree);
-		// 		r.right := newRight;
-		// 		if(newRight == n){
-		// 			n.parent := t;
-		// 		}
+			if (t.value == n.value) {
+				t.Repr := t.Repr + {n};
+				return;
+			}
 
 
-		// 		if(n.parent != null){
-		// 			ElemsRefTrans(n,newRight,r);
-		// 			if(n != newRight) {
-		// 				partialNoRRTrans(n.parent,newRight,r);
-		// 			}
-		// 		}
-		// 		return;
-		// 	}
-			
-		// 	assert(false);
+			// n.parent doesn't work because dafny doesn't know n remains the same
 
-		// }
+			if (n.value < t.value) {
+				label L1:
+				var newLeft := insertBST(t.left, n);
+
+				r.Repr := r.Repr + {n};
+				r.left := newLeft;
+				if(newLeft == n){
+					n.parent := t;
+				}
+				if(n.parent != null){
+					ElemsRefTrans(n,newLeft,r);
+					if(n != newLeft) {
+						partialNoRRTrans(n.parent,newLeft,r);
+					}
+				}
+				return;
+			}
+
+			if (n.value > t.value) {
+				label L2:
+				var newRight := insertBST(t.right, n);
+				r.Repr := r.Repr + {n};
+				r.right := newRight;
+				if(newRight == n){
+					n.parent := t;
+				}
+				if(n.parent != null){
+					ElemsRefTrans(n,newRight,r);
+					if(n != newRight) {
+						partialNoRRTrans(n.parent,newRight,r);
+					}
+				}
+				return;
+			}
+		}
 
 		// static method getGrandparent(t : RBTreeRef?) returns (g : RBTreeRef?)
 
 }
 
-// method Testing()
-// {
-// 	var t0 := Node(Red,10,(Node(Black,9,Empty,Empty)),Empty);
-// 	assert(!isWellFormed(t0));
-// 	var t1 := Node(Black,10,(Node(Red,9,Empty,Empty)),Empty);
-// 	assert(isWellFormed(t1));
+method Testing()
+{
+	var t2 := new RBTreeRef;
+	t2.value, t2.color, t2.right, t2.parent := 10, Black, null, null;
 
-// 	var t2 := new RBTreeRef;
-// 	t2.Tree := t1;
-// 	t2.value, t2.color, t2.right, t2.parent := 10, Black, null, null;
+	var t3 := new RBTreeRef;
+	t3.left := null;
+	t3.right := null;
+	t3.color := Red;
+	t3.parent := t2;
+	t3.value := 9;
 
-// 	var t3 := new RBTreeRef;
-// 	t3.Tree := Node(Red,9,Empty,Empty);
-// 	t3.left := null;
-// 	t3.right := null;
-// 	t3.color := Red;
-// 	t3.parent := t2;
-// 	t3.value := 9;
+	t2.Repr := {t2,t3}	;
+	t3.Repr := {t3};
+	t2.left := t3;
 
-// 	t2.Repr := {t2,t3}	;
-// 	t3.Repr := {t3};
-// 	t2.left := t3;
-
-// 	assert(t2.Valid());
+	assert(t2.Valid());
 
 
-// 	// Methods are opaque!!
-// 	var r := RBTreeRef.Member(t2, 9);
-// 	// assertion would fail if Member weren't annotated
-// 	assert(r);
-// }
-
-
-// predicate isBlack(t : RBTree) {
-// 	!isRed(t)
-// }
-
-// predicate method isRed(t : RBTree) {
-// 	t.Node? && t.color == Red
-// }
-
-
-// function countBlack(t : RBTree) : nat {
-// 	if t.Empty? then 1 else (if t.color == Red then countBlack(t.left) else 1 + countBlack(t.left))
-// }
-
-// predicate isBalanced(t : RBTree) {
-// 	if t.Empty? then true else
-// 		(countBlack(t.left) == countBlack(t.right) && isBalanced(t.left) && isBalanced(t.right))
-// }
-
-// predicate isOrdered(t : RBTree) {
-// 	if t.Empty? then true else
-// 		(forall i :: i in elems(t.left) ==> i < t.value) &&
-// 		(forall i :: i in elems(t.right) ==> i > t.value)
-// }
-
-// predicate isOrdered(t: RBTree) {
-// 	if t.Empty? then true else
-// 		(t.left.Node? ==> t.left.value < t.value && isOrdered(t.left)) &&
-// 		(t.right.Node? ==> t.value < t.right.value && isOrdered(t.right))
-// }
-
-
-// predicate noRedRedRP(t : RBTree) {
-// 	(isRed(t) ==> !isRed(t.right)) &&
-// 		(t.Node? ==> noRedRed(t.right))
-// }
-
-// predicate noRedRedLP(t : RBTree) {
-//   (isRed(t) ==> !isRed(t.left)) &&
-// 		(t.Node? ==> noRedRed(t.left))
-// }
-
-
-// predicate noRedRedR(t : RBTree) {
-// 	(isRed(t) ==> !isRed(t.left) && !isRed(t.right)) &&
-// 		(t.Node? ==> noRedRed(t.right))
-// }
-
-// predicate noRedRedL(t : RBTree) {
-//   (isRed(t) ==> !isRed(t.left) && !isRed(t.right)) &&
-// 		(t.Node? ==> noRedRed(t.left))
-// }
-
-// predicate noRedRed(t : RBTree) {
-// 	(isRed(t) ==> !isRed(t.left) && ! isRed(t.right)) &&
-// 		(t.Node? ==> noRedRed(t.left) && noRedRed(t.right))
-// }
-
-// predicate isWellFormed(t : RBTree) {
-// 	isBalanced(t) && isOrdered(t) && noRedRed(t)
-// }
-
-
-// predicate noRedRedExceptTop(t : RBTree) {
-// 	(t.Node? ==> noRedRed(t.left) && noRedRed(t.right))	
-// }
-
-// predicate almostWellFormed(t : RBTree) {
-// 	isBalanced(t) && isOrdered(t) && noRedRedExceptTop(t)
-// }
-
-
-
-// method ins(t : RBTree, v: int) returns (r : RBTree)
-// 	requires almostWellFormed(t)
-// 	ensures almostWellFormed(r)		// need to include more precise information about ordering
-// 	decreases t;
-// {
-// 	if(t.Empty?){
-// 		return Node(Red,v,Empty,Empty);
-// 	}
-// 	if (v < t.value) {
-		
-// 	}
-// 	if (v > t.value) {
-		
-// 	}
-// 	return t;
-// }
-
-// method setBlack(t : RBTree) returns (r : RBTree)
-// 	requires almostWellFormed(t)
-// 	ensures isWellFormed(r)
-// {
-// 	if (t.Empty?) {
-// 		return Empty;
-// 	}
-// 	return Node(Black, t.value,t.left,t.right);
-// }
-
-
-// method balanceL(c : Color, v : int, l : RBTree, r : RBTree) returns (r : RBTree)
-// 	requires 
-// {
-// }
-
-
-// method insert(t : RBTree) returns (r : RBTree)  {
-	
-
-// 	// r := Empty;
-// }
-
-// class RBTree {
-// 		ghost var Repr: set<RBTree>
-// 		var value: int
-// 		var left: RBTree?
-// 		var right: RBTree?
-
-// 		predicate Valid()
-// 			decreases Repr + {this}
-// 			reads this, Repr {
-// 				this in Repr &&
-// 					1 <= size &&
-// 					(left == null && right == null ==> size == 1) &&
-// 					(left == null && right != null ==> size == right.size + 1) &&
-// 					(left != null && right == null ==> size == left.size + 1) &&
-// 					(left != null && right != null ==> size == left.size + right.size + 1) &&
-// 					// ordering?
-// 					(left != null ==> left.Repr <= Repr && left.size < size && this !in left.Repr && left.Valid()) &&
-// 					(right != null ==> right.Repr <= Repr && right.size < size && this !in right.Repr && right.Valid())
-// 		}
-// }
-
-
-// class Node {
-//   // ghost var List: seq<int>
-//   ghost var Repr: set<Node>
-//   var head: int
-//   var next: Node? // Node? means a Node value or null
-// 	var parent: Node?
-
-//   predicate Valid()
-// 		decreases Repr
-//     reads this, Repr
-//   {
-//     this in Repr &&
-//     // 1 <= |List| && List[0] == head &&
-//     // (next == null ==> |List| == 1) &&
-//     (next != null ==>
-//       next in Repr && next.Repr <= Repr && this !in next.Repr &&
-//       next.Valid() && // && next.List == List[1..] 
-// 			(next.parent == this)) 
-			
-//   }
-
-//   // static method Cons(x: int, tail: Node?) returns (n: Node)
-//   //   requires tail == null || tail.Valid()
-//   //   ensures n.Valid()
-//   //   ensures if tail == null then n.List == [x]
-//   //                           else n.List == [x] + tail.List
-//   // {
-//   //   n := new Node;
-//   //   n.head, n.next := x, tail;
-//   //   if (tail == null) {
-//   //     n.List := [x];
-//   //     n.Repr := {n};
-//   //   } else {
-//   //     n.List := [x] + tail.List;
-//   //     n.Repr := {n} + tail.Repr;
-//   //   }
-//   // }
-// }
-
+	// Methods are opaque!!
+	var r := RBTreeRef.Member(t2, 9);
+	// assertion would fail if Member weren't annotated
+	assert(r);
+}
